Examples/EdmondsKarp_Maxflow/EdmondsKarp_Time.thy
@@ -3,9 +3,6 @@ theory EdmondsKarp_Time
  (*    "SepLogicTime_RBTreeBasic.Asymptotics_2D" 
       \<longrightarrow> Cannot join unrelated theory certificates SepLogicTime_RBTreeBasic.Asymptotics_2D:321 and SepLogicTime_RBTreeBasic.RBTree_Impl:4570
   *)
-
-  
-    "../../Refine_Imperative_HOL/IICF/Impl/IICF_RbtMap_Map"
 begin
  
 lemma "(\<lambda>x::nat. real ((3 ))) \<in> \<Theta>(\<lambda>(x). real 1)" 
